theories/SetModel/HO_model.v
@@ -7,8 +7,8 @@ Import ListNotations.
 Import CombineNotations.
 
 Require Import library.
-Require Import ZF_axioms ZF_library.
-Require Import HO HO_pi HO_sigma HO_nat.
+Require Import ZF_axioms ZF_library ZF_nat ZF_acc.
+Require Import HO HO_univ HO_prop HO_box HO_pi HO_sigma HO_nat HO_obseq HO_forall.
 
 Open Scope subst_scope.
 
@@ -18,50 +18,238 @@ Definition to_ZF_level (l : level) : nat :=
   | prop => 0
   end.
 
-Inductive interp_ctx : forall (Γ : ctx), ZFSet -> SProp :=
+Scheme typing_mutS := Induction for typing Sort Prop
+with ctx_typing_mutS := Induction for ctx_typing Sort Prop
+with conversion_mutS := Induction for conversion Sort Prop.
+Combined Scheme ctx_typing_conversion_mutindS from typing_mutS, ctx_typing_mutS, conversion_mutS.
 
-| interp_empty : interp_ctx ∙ (setSingl ∅)
+(* Interprétation comme des fonctions partielles
+   - [_] : ctx -> ZFSet
+   - [_ ⊢ _] : level -> tm -> ZFSet -> ZFSet *)
 
-| interp_cons  : forall Γ l A iΓ iA, interp_ctx Γ iΓ -> interp_tm Γ l A iA
-                 -> interp_ctx (Γ ,, (l , A)) (setSigma (to_ZF_level l) iΓ (fun γ => 𝕌el (to_ZF_level l) (iA γ)))
+Inductive interp_ctx : forall (Γ : ctx), ZFSet -> Prop :=
 
-with is_nth_proj : forall (Γ : ctx), (ZFSet -> ZFSet) -> SProp :=
-| here :
-  -> is_nth_proj (Γ ,, (l , A)) (fun γa => setSndSigma (to_ZF_level l) Γi (fun γ => 𝕌el (to_ZF_level l) (iA γ)) γa)
+| interp_empty : interp_ctx ∙ ⋆
 
-with interp_tm : forall (Γ : ctx) (l : level) (A : term), (ZFSet -> ZFSet) -> SProp :=
+| interp_cons_rel : forall Γ l A iΓ iA, interp_ctx Γ iΓ -> interp_tm Γ (Ax (ty l)) A iA
+                    -> interp_ctx (Γ ,, (ty l , A)) (ctxExt l iΓ (fun γ => 𝕌el l (iA γ)))
 
-| interp_pi : forall Γ lA lB A B iΓ iA iB, interp_tm Γ lA A iA
-              -> interp_tm (Γ ,, (lA , A)) (ty lB) B iB
-              -> interp_tm Γ (Ru lA (ty lB)) (Pi lA (ty lB) A B) (piTy_HO (to_ZF_level (Ru lA (ty lB))) iΓ iA (fun γ a => iB ⟨ γ ; a ⟩))
+| interp_cons_irr : forall Γ A iΓ iA, interp_ctx Γ iΓ -> interp_tm Γ (ty 0) A iA
+                    -> interp_ctx (Γ ,, (BasicAST.prop , A)) (ctxExt 0 iΓ iA)
 
-(* | interp_forall :  *)
+with nth_proj : forall (Γ : ctx) (l : level) (x : nat), (ZFSet -> ZFSet) -> Prop :=
 
-| interp_nat : forall Γ, interp_tm Γ (ty 0) Nat natTy_HO
+| here_rel : forall Γ l A iΓ iA, interp_ctx Γ iΓ -> interp_tm Γ (Ax (ty l)) A iA
+             -> nth_proj (Γ ,, (ty l , A)) (ty l) 0 (setSndSigma l iΓ (fun γ => 𝕌el l (iA γ)))
 
-| interp_type : forall Γ l, interp_tm Γ (Ax (ty l)) (Sort (ty l)) natTy_HO
+| there_rel : forall Γ l lA A x iΓ iA ix, interp_ctx Γ iΓ -> interp_tm Γ (Ax (ty lA)) A iA -> nth_proj Γ l x ix
+              -> nth_proj (Γ ,, (ty lA , A)) l (S x) (fun γa => ix (setFstSigma lA iΓ (fun γ => 𝕌el lA (iA γ)) γa))
 
-| interp_prop : forall Γ l, interp_tm Γ (Ax (ty l)) (Sort (ty l)) natTy_HO
+| here_irr : forall Γ A iΓ iA, interp_ctx Γ iΓ -> interp_tm Γ (ty 0) A iA
+             -> nth_proj (Γ ,, (BasicAST.prop , A)) BasicAST.prop 0 (setSndSigma 0 iΓ iA)
 
-(* | interp_acc : ... *)
+| there_irr : forall Γ l A x iΓ iA ix, interp_ctx Γ iΓ -> interp_tm Γ (ty 0) A iA -> nth_proj Γ l x ix
+              -> nth_proj (Γ ,, (BasicAST.prop , A)) l (S x) (fun γa => ix (setFstSigma 0 iΓ iA γa))
 
-| interp_
+with interp_tm : forall (Γ : ctx) (l : level) (A : term), (ZFSet -> ZFSet) -> Prop :=
 
-piTy_HO (n : nat) (Γ : ZFSet) (A : ZFSet -> ZFSet) (B : ZFSet -> ZFSet -> ZFSet) : ZFSet -> ZFSet :=
+| interp_var : forall Γ l x ix, nth_proj Γ l x ix
+               -> interp_tm Γ l (var x) ix
+
+| interp_type : forall Γ l, 
+                interp_tm Γ (Ax (Ax (ty l))) (Sort (ty l)) (univTy_HO l)
+
+| interp_prop : forall Γ, 
+                interp_tm Γ (ty 1) (Sort BasicAST.prop) propTy_HO
+
+| interp_pi_rr : forall Γ lA lB A B iA iB, interp_tm Γ (Ax (ty lA)) A iA
+                 -> interp_tm (Γ ,, (ty lA , A)) (Ax (ty lB)) B iB
+                 -> interp_tm Γ (Ax (Ru (ty lA) (ty lB))) (Pi (ty lA) (ty lB) A B) 
+                              (piTy_HO lA lB iA iB)
+
+| interp_pi_ir : forall Γ lB A B iA iB, interp_tm Γ (Ax BasicAST.prop) A iA
+                 -> interp_tm (Γ ,, (BasicAST.prop , A)) (Ax (ty lB)) B iB
+                 -> interp_tm Γ (Ax (ty lB)) (Pi BasicAST.prop (ty lB) A B)
+                              (piTy_HO 0 lB (boxTy_HO iA) iB)
+
+| interp_pi_ri : forall Γ lA A B iA iB, interp_tm Γ (Ax (ty lA)) A iA
+                 -> interp_tm (Γ ,, (ty lA , A)) (Ax BasicAST.prop) B iB
+                 -> interp_tm Γ (Ax BasicAST.prop) (Pi (ty lA) BasicAST.prop A B) 
+                              (forallTy_HO lA iA iB)
+
+| interp_pi_ii : forall Γ A B iA iB, interp_tm Γ (Ax BasicAST.prop) A iA
+                 -> interp_tm (Γ ,, (BasicAST.prop , A)) (Ax BasicAST.prop) B iB
+                 -> interp_tm Γ (Ax BasicAST.prop) (Pi BasicAST.prop BasicAST.prop A B)
+                              (forallTy_HO 0 (boxTy_HO iA) iB)
+
+| interp_lam_rr : forall Γ lA lB A B t iA it, interp_tm Γ (Ax (ty lA)) A iA
+                  -> interp_tm (Γ ,, (ty lA , A)) (ty lB) t it
+                  -> interp_tm Γ (Ru (ty lA) (ty lB)) (lam (ty lA) (ty lB) A B t) (lamTm_HO lA lB iA it)
+
+| interp_lam_ir : forall Γ lB A B t iA it, interp_tm Γ (Ax BasicAST.prop) A iA
+                  -> interp_tm (Γ ,, (BasicAST.prop , A)) BasicAST.prop t it
+                  -> interp_tm Γ (ty lB) (lam BasicAST.prop (ty lB) A B t) (lamTm_HO 0 lB (boxTy_HO iA) it)
+
+| interp_app_rr : forall Γ lA lB A B t u iA it iu, interp_tm Γ (Ax (ty lA)) A iA
+                  -> interp_tm Γ (Ru (ty lA) (ty lB)) t it
+                  -> interp_tm Γ (ty lA) u iu
+                  -> interp_tm Γ (ty lB) (app (ty lA) (ty lB) A B t u) (appTm_HO lA lB iA it iu)
+
+| interp_app_ir : forall Γ lB A B t u iA it iu, interp_tm Γ (Ax BasicAST.prop) A iA
+                  -> interp_tm Γ (ty lB) t it
+                  -> interp_tm Γ BasicAST.prop u iu
+                  -> interp_tm Γ (ty lB) (app BasicAST.prop (ty lB) A B t u) (appTm_HO 0 lB (boxTy_HO iA) it iu).
+
+(* | interp_nat : forall Γ, *)
+(*                interp_tm Γ (ty 1) Nat natTy_HO *)
+
+(* | interp_zero : forall Γ, *)
+(*                 interp_tm Γ (ty 0) zero zeroTm_HO *)
+
+(* | interp_succ : forall Γ t it, interp_tm Γ (ty 0) t it *)
+(*                 -> interp_tm Γ (ty 0) (succ t) (sucTm_HO it) *)
+
+(* | interp_natrec : *)
+
+(* | interp_acc : *)
+
+(* | interp_accelim : *)
+
+(* | interp_obseq : *)
+
+(* | interp_cast : *)
 
 
 
-with interp_tm : forall (Γ : ctx) (l : level) (t : term), (ZFSet -> ZFSet) -> SProp :=
-| interp_var : is_nth_proj Γ π 
-    -> interp_tm Γ l (var x) π
+(* Interprétation des renommages et des substitutions *)
 
 
+(* Fonction partielle (?) *)
 
-Γ ⊢ t : A
 
-∀ γ ∈ ⟦ Γ ⟧, ⟦ Γ ⊢ t ⟧γ ∈ ⟦ Γ ⊢ A ⟧γ
+(* Lemme fondamental *)
 
-Lemma model : forall Γ l t A, Γ ⊢< l > t : A -> True.
+Inductive model_ctx (Γ : ctx) : Prop :=
+| mkModelCtx (iΓ : ZFSet) (fΓ : interp_ctx Γ iΓ).
 
-(forall Γ l t A, Γ ⊢< l > t : A -> forall k (_temp : l = ty k), Γ ⊢< l > t ≡ t : A -> Γ ⊨< l > t ≡ t : A) ∧
-      (forall Γ l t u A, Γ ⊢< l > t ≡ u : A -> forall k (_temp : l = ty k), Γ ⊢< l > t ≡ u : A -> Γ ⊨< l > t ≡ u : A).
+Inductive model_typing_rel (Γ : ctx) (l : nat) (t A : term) : Prop :=
+| mkModelTypingRel (iΓ : ZFSet)
+    (fΓ : interp_ctx Γ iΓ)
+    (iA : ZFSet -> ZFSet)
+    (fA : interp_tm Γ (Ax (ty l)) A iA)
+    (it : ZFSet -> ZFSet)
+    (ft : interp_tm Γ (ty l) t it)
+    (vA : ∀ γ ∈ iΓ, iA γ ∈ 𝕌 l)
+    (vt : ∀ γ ∈ iΓ, it γ ∈ 𝕌el l (iA γ)).
+
+Inductive model_typing_irr (Γ : ctx) (t A : term) : Prop :=
+| mkModelTypingIrr (iΓ : ZFSet)
+    (fΓ : interp_ctx Γ iΓ)
+    (iA : ZFSet -> ZFSet)
+    (fA : interp_tm Γ (Ax BasicAST.prop) A iA)
+    (vA : ∀ γ ∈ iΓ, iA γ ∈ Ω)
+    (vt : ∀ γ ∈ iΓ, ∅ ∈ iA γ).
+
+Definition model_typing (Γ : ctx) (l : level) (t A : term) : Prop :=
+  match l with
+  | BasicAST.prop => model_typing_irr Γ t A
+  | ty l => model_typing_rel Γ l t A
+  end.
+
+Inductive model_conv_rel (Γ : ctx) (l : nat) (t u A : term) : Prop :=
+| mkModelConvRel (iΓ : ZFSet)
+    (fΓ : interp_ctx Γ iΓ)
+    (iA : ZFSet -> ZFSet)
+    (fA : interp_tm Γ (Ax (ty l)) A iA)
+    (it : ZFSet -> ZFSet)
+    (ft : interp_tm Γ (ty l) t it)
+    (iu : ZFSet -> ZFSet)
+    (fu : interp_tm Γ (ty l) u iu)
+    (* (vA : ∀ γ ∈ iΓ, iA γ ∈ 𝕌 l) *)
+    (* (vt : ∀ γ ∈ iΓ, it γ ∈ 𝕌el l (iA γ)) *)
+    (vu : ∀ γ ∈ iΓ, it γ ≡ iu γ).
+  
+Inductive model_conv_irr (Γ : ctx) (t u A : term) : Prop := True.
+(* | mkModelConvIrr (iΓ : ZFSet) *)
+(*     (fΓ : interp_ctx Γ iΓ) *)
+(*     (iA : ZFSet -> ZFSet) *)
+(*     (fA : interp_tm Γ (Ax BasicAST.prop) A iA) *)
+(*     (vA : ∀ γ ∈ iΓ, iA γ ∈ Ω) *)
+(*     (vt : ∀ γ ∈ iΓ, ∅ ∈ iA γ). *)
+
+Definition model_conv (Γ : ctx) (l : level) (t u A : term) : Prop :=
+  match l with
+  | BasicAST.prop => model_conv_irr Γ t u A
+  | ty l => model_conv_rel Γ l t u A
+  end.
+
+(* We assume that the extra assumptions are validated by the model *)
+Axiom model_assm : forall c A iA, nth_error assm_sig c = Some A
+                                  -> interp_tm ∙ (ty 0) A iA
+                                  -> ∅ ∈ iA ∅.
+
+Theorem model : (forall Γ l t A, Γ ⊢< l > t : A -> model_typing Γ l t A) 
+              /\ (forall Γ, ⊢ Γ -> model_ctx Γ)
+              /\ (forall Γ l t u A, Γ ⊢< l > t ≡ u : A -> model_conv Γ l t u A).
+Proof.
+  apply ctx_typing_conversion_mutindS.
+  - admit.
+  - intros Γ l tΓ [ iΓ fΓ ]. destruct l as [ l | ].
+    + econstructor.
+      * exact fΓ.
+      * apply interp_type.
+      * apply interp_type.
+      * apply univTy_HO_typing.
+      * apply univTy_HO_typing'.
+    + econstructor.
+      * exact fΓ.
+      * apply interp_type.
+      * apply interp_prop.
+      * apply univTy_HO_typing.
+      * apply propTy_HO_typing'.
+  - intros Γ c A tΓ [ iΓ fΓ ] Hc tA [ iΓ' fΓ' iΩ fΩ iA fA vΩ vA ]. econstructor.
+    * exact fΓ.
+    * assert (interp_tm Γ (Ax BasicAST.prop) A (fun _ => iA ∅)) as H. admit. exact H. (* weakening of interpretation *)
+    * intros γ Hγ. cbn. admit.  (* some massaging is in order here *)
+    * intros γ Hγ. now apply (model_assm c A).
+  - intros Γ i j A B tA [ iΓ fΓ iS fS iA fA vS vA ] tB [ iΓ' fΓ' iT fT iB fB vT vB ].
+    destruct i as [ i | ] ; destruct j as [ j | ] ; cbn in *.
+    + econstructor.
+      * exact fΓ.
+      * apply interp_type.
+      * apply interp_pi_rr. exact fA. exact fB.
+      * apply univTy_HO_typing.
+      *
+
+Admitted.
+
+Corollary consistency : forall t , ∙ ⊢< BasicAST.prop > t : Pi (ty 0) BasicAST.prop (Sort BasicAST.prop) (var 0) -> False.
+Proof.
+  (* We interpret the judgment in our ZF model *)
+  intros t H. apply model in H. destruct H as [ iΓ fΓ iA fA _ vt ].
+  (* We unfold the interpretation function using [inversion] *)
+  inversion fΓ. destruct H0. clear fΓ.
+  inversion fA. symmetry in H1. destruct H1. symmetry in H. destruct H.
+  symmetry in H0. destruct H0. symmetry in H2. destruct H2. destruct H4. clear fA.
+  inversion H3. symmetry in H. destruct H. destruct H2. clear H3.
+  inversion H5. symmetry in H0. destruct H0. symmetry in H1. destruct H1.
+  symmetry in H. destruct H. destruct H3. clear H5.
+  inversion H2. symmetry in H. destruct H. symmetry in H0. destruct H0.
+  symmetry in H3. destruct H3. destruct H5. clear H2.
+  inversion H1. destruct H0. clear H1.
+  inversion H4. symmetry in H. destruct H. destruct H2. clear H4.
+  (* We derive a contradiction *)
+  assert (∅ ∈ ⋆) as Hγ. { now apply inSetSingl. }
+  specialize (vt _ Hγ). clear Hγ. apply prop_true_if in vt.
+  assert (∅ ∈ 𝕌el 0 (propTy_HO ∅)) as Hp.
+  { refine (transpS (fun X => ∅ ∈ X) (sym el_propTy) _).
+    apply ZFinpower. intros x Hx. apply ZFinempty in Hx. destruct Hx. }
+  specialize (vt _ Hp). assert (∅ ∈ ∅).
+  { refine (transpS (fun X => ∅ ∈ X) _ vt). apply setSigmaβ2.
+    - intros γ Hγ. apply 𝕌el_typing. now apply (propTy_HO_typing (Γ := ⋆)).
+    - now apply inSetSingl.
+    - exact Hp. }
+  apply ZFinempty in H. destruct H.
+Qed.
+
+Print Assumptions consistency.
