theories/SetModel/HO_pi.v
@@ -1,149 +1,261 @@
+From Stdlib Require Import Arith.
 Require Import library.
 Require Import ZF_axioms ZF_library ZF_nat.
-Require Import HO.
+Require Import HO HO_univ.
 
 (* Pi types *)
 
-Definition piTy_HO (n : nat) (A : ZFSet -> ZFSet) (B : ZFSet -> ZFSet) : ZFSet -> ZFSet :=
-  fun γ => ⟨ setPi n (𝕌el n (A γ)) (fun a => 𝕌el n (B ⟨ γ ; a ⟩))
-           ; ⟨ ZFone ; typeTelescope2 n A B γ ⟩ ⟩.
+Definition piTy_HO (nA nB : nat) (A : ZFSet -> ZFSet) (B : ZFSet -> ZFSet) : ZFSet -> ZFSet :=
+  fun γ => ⟨ setPi (max nA nB) (𝕌el nA (A γ)) (fun a => 𝕌el nB (B ⟨ γ ; a ⟩))
+           ; ⟨ ZFone ; typeTelescope2 nA nB A B γ ⟩ ⟩.
 
-Lemma piTy_HO_typing {n : nat} {Γ : ZFSet} {A : ZFSet -> ZFSet} {B : ZFSet -> ZFSet}
-  (HA : ∀ γ ∈ Γ, A γ ∈ 𝕌 n) (HB : ∀ γa ∈ ctxExt n Γ A, B γa ∈ 𝕌 n) :
-  ∀ γ ∈ Γ, piTy_HO n A B γ ∈ 𝕌 n.
+Lemma piTy_HO_typing {nA nB : nat} {Γ : ZFSet} {A : ZFSet -> ZFSet} {B : ZFSet -> ZFSet}
+  (HA : ∀ γ ∈ Γ, A γ ∈ 𝕌 nA) (HB : ∀ γa ∈ ctxExt nA Γ A, B γa ∈ 𝕌 nB) :
+  ∀ γ ∈ Γ, piTy_HO nA nB A B γ ∈ 𝕌 (max nA nB).
 Proof.
   intros γ Hγ. cbn. apply setMkPair_typing.
   - apply setPi_typing.
-    + apply 𝕌el_typing. now apply HA.
-    + intros a Ha. apply 𝕌el_typing. now apply (typeExt_typing HA HB). 
+    + eapply univ_le_incl. apply Nat.le_max_l. apply 𝕌el_typing. now apply HA.
+    + intros a Ha. eapply univ_le_incl. apply Nat.le_max_r. apply 𝕌el_typing. now apply (typeExt_typing HA HB). 
   - apply setMkPair_typing.
     + apply one_typing.
-    + apply (typeTelescope2_typing n (Γ := Γ)) ; try assumption. 
+    + apply (typeTelescope2_typing nA nB (Γ := Γ)) ; try assumption. 
 Qed.
 
-Lemma el_piTy {n : nat} {Γ γ : ZFSet} {A : ZFSet -> ZFSet} {B : ZFSet -> ZFSet}
-  (HA : ∀ γ ∈ Γ, A γ ∈ 𝕌 n) (HB : ∀ γa ∈ ctxExt n Γ A, B γa ∈ 𝕌 n) (Hγ : γ ∈ Γ) :
-  𝕌el n (piTy_HO n A B γ) ≡ setPi n (𝕌el n (A γ)) (fun a => 𝕌el n (B ⟨ γ ; a ⟩)).
+Lemma piTy_HO_typing' {nA nB : nat} {Γ : ZFSet} {A : ZFSet -> ZFSet} {B : ZFSet -> ZFSet}
+  (HA : ∀ γ ∈ Γ, A γ ∈ 𝕌 nA) (HB : ∀ γa ∈ ctxExt nA Γ A, B γa ∈ 𝕌 nB) :
+  ∀ γ ∈ Γ, piTy_HO nA nB A B γ ∈ 𝕌el (S (max nA nB)) (univTy_HO (max nA nB) γ).
+Proof.
+  intros γ Hγ. refine (transpS (fun X => _ ∈ X) (sym _) (piTy_HO_typing HA HB γ Hγ)).
+  now apply el_univTy.
+Qed.
+
+Lemma el_piTy {nA nB : nat} {Γ γ : ZFSet} {A : ZFSet -> ZFSet} {B : ZFSet -> ZFSet} 
+  (HA : ∀ γ ∈ Γ, A γ ∈ 𝕌 nA) (HB : ∀ γa ∈ ctxExt nA Γ A, B γa ∈ 𝕌 nB) (Hγ : γ ∈ Γ) :
+  𝕌el (max nA nB) (piTy_HO nA nB A B γ) ≡ setPi (max nA nB) (𝕌el nA (A γ)) (fun a => 𝕌el nB (B ⟨ γ ; a ⟩)).
 Proof.
   apply setPairβ1'. now apply (piTy_HO_typing (Γ := Γ)).
 Qed.
 
-Lemma hd_piTy {n : nat} {Γ γ : ZFSet} {A : ZFSet -> ZFSet} {B : ZFSet -> ZFSet}
-  (HA : ∀ γ ∈ Γ, A γ ∈ 𝕌 n) (HB : ∀ γa ∈ ctxExt n Γ A, B γa ∈ 𝕌 n) (Hγ : γ ∈ Γ) :
-  𝕌hd n (piTy_HO n A B γ) ≡ ZFone.
+Lemma el_piTy' {n nA nB : nat} {Γ γ : ZFSet} {A : ZFSet -> ZFSet} {B : ZFSet -> ZFSet} 
+  (HnA : nA <= n) (HnB : nB <= n) (HA : ∀ γ ∈ Γ, A γ ∈ 𝕌 nA) (HB : ∀ γa ∈ ctxExt nA Γ A, B γa ∈ 𝕌 nB) (Hγ : γ ∈ Γ) :
+  𝕌el n (piTy_HO nA nB A B γ) ≡ setPi (max nA nB) (𝕌el nA (A γ)) (fun a => 𝕌el nB (B ⟨ γ ; a ⟩)).
+Proof.
+  apply setPairβ1'. eapply 𝕌_le_incl. apply (Nat.max_lub _ _ _ HnA HnB). now apply (piTy_HO_typing (Γ := Γ)).
+Qed.
+
+Lemma hd_piTy' {n nA nB : nat} {Γ γ : ZFSet} {A : ZFSet -> ZFSet} {B : ZFSet -> ZFSet} 
+  (HnA : nA <= n) (HnB : nB <= n) (HA : ∀ γ ∈ Γ, A γ ∈ 𝕌 nA) (HB : ∀ γa ∈ ctxExt nA Γ A, B γa ∈ 𝕌 nB) (Hγ : γ ∈ Γ) :
+  𝕌hd n (piTy_HO nA nB A B γ) ≡ ZFone.
 Proof.
   refine (trans (fequal (setFstPair ω (𝕍 n)) _) _).
-  apply setPairβ2'. now apply (piTy_HO_typing (Γ := Γ)).
-  apply setPairβ1. apply one_typing. apply (typeTelescope2_typing n (Γ := Γ)) ; try assumption.
+  apply setPairβ2'. eapply 𝕌_le_incl. apply (Nat.max_lub _ _ _ HnA HnB). now apply (piTy_HO_typing (Γ := Γ)).
+  apply setPairβ1. apply one_typing. eapply univ_le_incl. apply (Nat.max_lub _ _ _ HnA HnB).
+  apply (typeTelescope2_typing nA nB (Γ := Γ)) ; try assumption.
 Qed.  
 
-Lemma lbl_piTy {n : nat} {Γ γ : ZFSet} {A : ZFSet -> ZFSet} {B : ZFSet -> ZFSet}
-  (HA : ∀ γ ∈ Γ, A γ ∈ 𝕌 n) (HB : ∀ γa ∈ ctxExt n Γ A, B γa ∈ 𝕌 n) (Hγ : γ ∈ Γ) :
-  𝕌lbl n (piTy_HO n A B γ) ≡ typeTelescope2 n A B γ.
+Lemma lbl_piTy' {n nA nB : nat} {Γ γ : ZFSet} {A : ZFSet -> ZFSet} {B : ZFSet -> ZFSet}
+  (HnA : nA <= n) (HnB : nB <= n) (HA : ∀ γ ∈ Γ, A γ ∈ 𝕌 nA) (HB : ∀ γa ∈ ctxExt nA Γ A, B γa ∈ 𝕌 nB) (Hγ : γ ∈ Γ) :
+  𝕌lbl n (piTy_HO nA nB A B γ) ≡ typeTelescope2 nA nB A B γ.
 Proof.
   refine (trans (fequal (setSndPair ω (𝕍 n)) _) _).
-  apply setPairβ2'. now apply (piTy_HO_typing (Γ := Γ)).
-  apply setPairβ2. apply one_typing. apply (typeTelescope2_typing n (Γ := Γ)) ; try assumption.
+  apply setPairβ2'. eapply 𝕌_le_incl. apply (Nat.max_lub _ _ _ HnA HnB). now apply (piTy_HO_typing (Γ := Γ)).
+  apply setPairβ2. apply one_typing. eapply univ_le_incl. apply (Nat.max_lub _ _ _ HnA HnB).
+  apply (typeTelescope2_typing nA nB (Γ := Γ)) ; try assumption.
 Qed.
 
-(* Injectivity of Pi types *)
+(* Recovering the domain and codomain, along with their levels, from the code of a Pi type *)
 
-Definition dom_piTy (n : nat) (x : ZFSet) :=
-  setFstPair (𝕌 n) (𝕍 n) (𝕌lbl n x).
+Definition dom_piTy (n : nat) (x : ZFSet) := setFstPair (ω × 𝕌 n) (ω × 𝕍 n) (𝕌lbl n x).
+Definition dom_piTy_level (n : nat) (x : ZFSet) := setFstPair ω (𝕌 n) (dom_piTy n x).
+Definition dom_piTy_set (n : nat) (x : ZFSet) := setSndPair ω (𝕌 n) (dom_piTy n x).
+Definition cod_piTy (n : nat) (x : ZFSet) := setSndPair (ω × 𝕌 n) (ω × 𝕍 n) (𝕌lbl n x).
+Definition cod_piTy_level (n : nat) (x : ZFSet) := setFstPair ω (𝕍 n) (cod_piTy n x).
+Definition cod_piTy_set (n : nat) (x : ZFSet) := setSndPair ω (𝕍 n) (cod_piTy n x).
 
-Definition cod_piTy (n : nat) (x : ZFSet) :=
-  setSndPair (𝕌 n) (𝕍 n) (𝕌lbl n x).
-
-Lemma dom_piTy_eq {n : nat} {Γ γ : ZFSet} {A : ZFSet -> ZFSet} {B : ZFSet -> ZFSet}
-  (HA : ∀ γ ∈ Γ, A γ ∈ 𝕌 n) (HB : ∀ γa ∈ ctxExt n Γ A, B γa ∈ 𝕌 n) (Hγ : γ ∈ Γ) :
-  dom_piTy n (piTy_HO n A B γ) ≡ A γ.
+Lemma dom_piTy_eq {nA nB n : nat} {Γ γ : ZFSet} {A : ZFSet -> ZFSet} {B : ZFSet -> ZFSet}
+  (HnA : nA <= n) (HnB : nB <= n) (HA : ∀ γ ∈ Γ, A γ ∈ 𝕌 nA) (HB : ∀ γa ∈ ctxExt nA Γ A, B γa ∈ 𝕌 nB) (Hγ : γ ∈ Γ) :
+  dom_piTy n (piTy_HO nA nB A B γ) ≡ ⟨ nat_to_ω nA ; A γ ⟩.
 Proof.
-  refine (trans (fequal (setFstPair (𝕌 n) (𝕍 n)) _) _).
-  now apply (lbl_piTy (Γ := Γ)). apply setPairβ1. now apply HA.
-  apply typeToGraph_sorting. now apply HA. now apply (typeExt_typing HA HB).
+  refine (trans (fequal (setFstPair (ω × 𝕌 n) (ω × 𝕍 n)) _) _). now apply (lbl_piTy' (Γ := Γ)). apply setPairβ1. 
+  - apply setMkPair_typing.
+    + apply nat_to_ω_typing.
+    + eapply 𝕌_le_incl. exact HnA. now apply HA.
+  - apply setMkPair_typing.
+    + apply nat_to_ω_typing.
+    + eapply univ_le_incl. apply (Nat.max_lub _ _ _ HnA HnB).
+      apply typeToGraph_sorting. now apply HA. now apply (typeExt_typing HA HB).
 Qed.
 
-Lemma cod_piTy_eq {n : nat} {Γ γ : ZFSet} {A : ZFSet -> ZFSet} {B : ZFSet -> ZFSet}
-  (HA : ∀ γ ∈ Γ, A γ ∈ 𝕌 n) (HB : ∀ γa ∈ ctxExt n Γ A, B γa ∈ 𝕌 n) (Hγ : γ ∈ Γ) :
-  cod_piTy n (piTy_HO n A B γ) ≡ typeToGraph n (A γ) (fun a => B ⟨ γ ; a ⟩).
+Lemma dom_piTy_level_eq {nA nB n : nat} {Γ γ : ZFSet} {A : ZFSet -> ZFSet} {B : ZFSet -> ZFSet}
+  (HnA : nA <= n) (HnB : nB <= n) (HA : ∀ γ ∈ Γ, A γ ∈ 𝕌 nA) (HB : ∀ γa ∈ ctxExt nA Γ A, B γa ∈ 𝕌 nB) (Hγ : γ ∈ Γ) :
+  dom_piTy_level n (piTy_HO nA nB A B γ) ≡ nat_to_ω nA.
 Proof.
-  refine (trans (fequal (setSndPair (𝕌 n) (𝕍 n)) _) _).
-  now apply (lbl_piTy (Γ := Γ)). apply setPairβ2. now apply HA.
-  apply typeToGraph_sorting. now apply HA. now apply (typeExt_typing HA HB).
+  refine (trans (fequal (setFstPair ω (𝕌 n)) _) _). now apply (dom_piTy_eq HnA HnB HA HB). apply setPairβ1.
+  - apply nat_to_ω_typing.
+  - eapply 𝕌_le_incl. exact HnA. now apply HA.
 Qed.
 
-Lemma piTy_HO_inj1 {n : nat} {Γ γ : ZFSet} {A A' B B' : ZFSet -> ZFSet} 
-  (HA : ∀ γ ∈ Γ, A γ ∈ 𝕌 n) (HB : ∀ γa ∈ ctxExt n Γ A, B γa ∈ 𝕌 n)
-  (HA' : ∀ γ ∈ Γ, A' γ ∈ 𝕌 n) (HB' : ∀ γa ∈ ctxExt n Γ A', B' γa ∈ 𝕌 n)
-  (Hγ : γ ∈ Γ) (H : piTy_HO n A B γ ≡ piTy_HO n A' B' γ) : A γ ≡ A' γ.
+Lemma dom_piTy_set_eq {nA nB n : nat} {Γ γ : ZFSet} {A : ZFSet -> ZFSet} {B : ZFSet -> ZFSet}
+  (HnA : nA <= n) (HnB : nB <= n) (HA : ∀ γ ∈ Γ, A γ ∈ 𝕌 nA) (HB : ∀ γa ∈ ctxExt nA Γ A, B γa ∈ 𝕌 nB) (Hγ : γ ∈ Γ) :
+  dom_piTy_set n (piTy_HO nA nB A B γ) ≡ A γ.
 Proof.
-  refine (trans (b := dom_piTy n (piTy_HO n A B γ)) _ _).
-  { symmetry. now apply (dom_piTy_eq (Γ := Γ)). }
-  refine (trans (fequal (dom_piTy n) H) _). now apply (dom_piTy_eq (Γ := Γ)).
+  refine (trans (fequal (setSndPair ω (𝕌 n)) _) _). now apply (dom_piTy_eq HnA HnB HA HB). apply setPairβ2.
+  - apply nat_to_ω_typing.
+  - eapply 𝕌_le_incl. exact HnA. now apply HA.
 Qed.
 
-Lemma piTy_HO_inj2' {n : nat} {Γ γ : ZFSet} {A A' B B' : ZFSet -> ZFSet} 
-  (HA : ∀ γ ∈ Γ, A γ ∈ 𝕌 n) (HB : ∀ γa ∈ ctxExt n Γ A, B γa ∈ 𝕌 n)
-  (HA' : ∀ γ ∈ Γ, A' γ ∈ 𝕌 n) (HB' : ∀ γa ∈ ctxExt n Γ A', B' γa ∈ 𝕌 n)
-  (Hγ : γ ∈ Γ) (H : piTy_HO n A B γ ≡ piTy_HO n A' B' γ) :
-  typeToGraph n (A γ) (fun a => B ⟨ γ ; a ⟩) ≡ typeToGraph n (A γ) (fun a => B' ⟨ γ ; a ⟩).
+Lemma cod_piTy_eq {n nA nB : nat} {Γ γ : ZFSet} {A : ZFSet -> ZFSet} {B : ZFSet -> ZFSet}
+  (HnA : nA <= n) (HnB : nB <= n) (HA : ∀ γ ∈ Γ, A γ ∈ 𝕌 nA) (HB : ∀ γa ∈ ctxExt nA Γ A, B γa ∈ 𝕌 nB) (Hγ : γ ∈ Γ) :
+  cod_piTy n (piTy_HO nA nB A B γ) ≡ ⟨ nat_to_ω nB ; typeToGraph nA nB (A γ) (fun a => B ⟨ γ ; a ⟩) ⟩.
 Proof.
-  pose proof (piTy_HO_inj1 HA HB HA' HB' Hγ H) as HAA'.
-  refine (trans (b := cod_piTy n (piTy_HO n A B γ)) _ _).
-  symmetry. now apply (cod_piTy_eq (Γ := Γ)). refine (trans (fequal (cod_piTy n) H) _).
-  refine (transpS (fun X => _ ≡ typeToGraph n X _) (sym HAA') _).
-  now apply (cod_piTy_eq (Γ := Γ)).
+  refine (trans (fequal (setSndPair (ω × 𝕌 n) (ω × 𝕍 n)) _) _). now apply (lbl_piTy' (Γ := Γ)). apply setPairβ2.
+  - apply setMkPair_typing.
+    + apply nat_to_ω_typing.
+    + eapply 𝕌_le_incl. exact HnA. now apply HA.
+  - apply setMkPair_typing.
+    + apply nat_to_ω_typing.
+    + eapply univ_le_incl. apply (Nat.max_lub _ _ _ HnA HnB).
+      apply typeToGraph_sorting. now apply HA. now apply (typeExt_typing HA HB).
 Qed.
 
-Lemma piTy_HO_inj2 {n : nat} {Γ γ a : ZFSet} {A A' B B' : ZFSet -> ZFSet} 
-  (HA : ∀ γ ∈ Γ, A γ ∈ 𝕌 n) (HB : ∀ γa ∈ ctxExt n Γ A, B γa ∈ 𝕌 n)
-  (HA' : ∀ γ ∈ Γ, A' γ ∈ 𝕌 n) (HB' : ∀ γa ∈ ctxExt n Γ A', B' γa ∈ 𝕌 n)
-  (Hγ : γ ∈ Γ) (H : piTy_HO n A B γ ≡ piTy_HO n A' B' γ) (Ha : a ∈ 𝕌el n (A γ)) :
+Lemma cod_piTy_level_eq {nA nB n : nat} {Γ γ : ZFSet} {A : ZFSet -> ZFSet} {B : ZFSet -> ZFSet}
+  (HnA : nA <= n) (HnB : nB <= n) (HA : ∀ γ ∈ Γ, A γ ∈ 𝕌 nA) (HB : ∀ γa ∈ ctxExt nA Γ A, B γa ∈ 𝕌 nB) (Hγ : γ ∈ Γ) :
+  cod_piTy_level n (piTy_HO nA nB A B γ) ≡ nat_to_ω nB.
+Proof.
+  refine (trans (fequal (setFstPair ω (𝕍 n)) _) _). now apply (cod_piTy_eq HnA HnB HA HB). apply setPairβ1.
+  - apply nat_to_ω_typing.
+  - eapply univ_le_incl. apply (Nat.max_lub _ _ _ HnA HnB).
+    apply typeToGraph_sorting. now apply HA. now apply (typeExt_typing HA HB).
+Qed.
+
+Lemma cod_piTy_set_eq {nA nB n : nat} {Γ γ : ZFSet} {A : ZFSet -> ZFSet} {B : ZFSet -> ZFSet}
+  (HnA : nA <= n) (HnB : nB <= n) (HA : ∀ γ ∈ Γ, A γ ∈ 𝕌 nA) (HB : ∀ γa ∈ ctxExt nA Γ A, B γa ∈ 𝕌 nB) (Hγ : γ ∈ Γ) :
+  cod_piTy_set n (piTy_HO nA nB A B γ) ≡ typeToGraph nA nB (A γ) (fun a => B ⟨ γ ; a ⟩).
+Proof.
+  refine (trans (fequal (setSndPair ω (𝕍 n)) _) _). now apply (cod_piTy_eq HnA HnB HA HB). apply setPairβ2.
+  - apply nat_to_ω_typing.
+  - eapply univ_le_incl. apply (Nat.max_lub _ _ _ HnA HnB).
+    apply typeToGraph_sorting. now apply HA. now apply (typeExt_typing HA HB).
+Qed.
+
+(* We deduce that Pi types are injective *)
+
+Definition maxmax (nA nA' nB nB' : nat) := max (max nA nA') (max nB nB').
+
+Lemma maxmax_le (nA nA' nB nB' : nat) :
+  (nA <= maxmax nA nA' nB nB') /\ (nA' <= maxmax nA nA' nB nB') /\ (nB <= maxmax nA nA' nB nB') /\ (nB' <= maxmax nA nA' nB nB').
+Proof.
+  split. { etransitivity. apply (Nat.le_max_l nA nA'). apply Nat.le_max_l. }
+  split. { etransitivity. apply (Nat.le_max_r nA nA'). apply Nat.le_max_l. }
+  split. { etransitivity. apply (Nat.le_max_l nB nB'). apply Nat.le_max_r. }
+  etransitivity. apply (Nat.le_max_r nB nB'). apply Nat.le_max_r.
+Qed.
+
+Lemma piTy_HO_inj_dom {nA nA' nB nB' : nat} {Γ γ : ZFSet} {A A' B B' : ZFSet -> ZFSet} 
+  (HA : ∀ γ ∈ Γ, A γ ∈ 𝕌 nA) (HB : ∀ γa ∈ ctxExt nA Γ A, B γa ∈ 𝕌 nB)
+  (HA' : ∀ γ ∈ Γ, A' γ ∈ 𝕌 nA') (HB' : ∀ γa ∈ ctxExt nA' Γ A', B' γa ∈ 𝕌 nB')
+  (Hγ : γ ∈ Γ) (H : piTy_HO nA nB A B γ ≡ piTy_HO nA' nB' A' B' γ) : A γ ≡ A' γ.
+Proof.
+  set (N := maxmax nA nA' nB nB').
+  refine (trans (b := dom_piTy_set N (piTy_HO nA nB A B γ)) _ _).
+  { symmetry. refine (dom_piTy_set_eq _ _ HA HB Hγ) ; now apply (maxmax_le nA nA' nB nB'). }
+  refine (trans (fequal (dom_piTy_set N) H) _).
+  refine (dom_piTy_set_eq _ _ HA' HB' Hγ) ; now apply (maxmax_le nA nA' nB nB').
+Qed.
+
+Lemma piTy_HO_inj_dom_level {nA nA' nB nB' : nat} {Γ γ : ZFSet} {A A' B B' : ZFSet -> ZFSet} 
+  (HA : ∀ γ ∈ Γ, A γ ∈ 𝕌 nA) (HB : ∀ γa ∈ ctxExt nA Γ A, B γa ∈ 𝕌 nB)
+  (HA' : ∀ γ ∈ Γ, A' γ ∈ 𝕌 nA') (HB' : ∀ γa ∈ ctxExt nA' Γ A', B' γa ∈ 𝕌 nB')
+  (Hγ : γ ∈ Γ) (H : piTy_HO nA nB A B γ ≡ piTy_HO nA' nB' A' B' γ) : nA ≡ nA'.
+Proof.
+  apply nat_to_ω_inj. set (N := maxmax nA nA' nB nB').
+  refine (trans (b := dom_piTy_level N (piTy_HO nA nB A B γ)) _ _).
+  { symmetry. refine (dom_piTy_level_eq _ _ HA HB Hγ) ; now apply (maxmax_le nA nA' nB nB'). }
+  refine (trans (fequal (dom_piTy_level N) H) _).
+  refine (dom_piTy_level_eq _ _ HA' HB' Hγ) ; now apply (maxmax_le nA nA' nB nB').
+Qed.
+
+Lemma piTy_HO_inj_cod_level {nA nA' nB nB' : nat} {Γ γ : ZFSet} {A A' B B' : ZFSet -> ZFSet} 
+  (HA : ∀ γ ∈ Γ, A γ ∈ 𝕌 nA) (HB : ∀ γa ∈ ctxExt nA Γ A, B γa ∈ 𝕌 nB)
+  (HA' : ∀ γ ∈ Γ, A' γ ∈ 𝕌 nA') (HB' : ∀ γa ∈ ctxExt nA' Γ A', B' γa ∈ 𝕌 nB')
+  (Hγ : γ ∈ Γ) (H : piTy_HO nA nB A B γ ≡ piTy_HO nA' nB' A' B' γ) : nB ≡ nB'.
+Proof.
+  apply nat_to_ω_inj. set (N := maxmax nA nA' nB nB').
+  refine (trans (b := cod_piTy_level N (piTy_HO nA nB A B γ)) _ _).
+  { symmetry. refine (cod_piTy_level_eq _ _ HA HB Hγ) ; now apply (maxmax_le nA nA' nB nB'). }
+  refine (trans (fequal (cod_piTy_level N) H) _).
+  refine (cod_piTy_level_eq _ _ HA' HB' Hγ) ; now apply (maxmax_le nA nA' nB nB').
+Qed.
+
+Lemma piTy_HO_inj_cod' {nA nA' nB nB' : nat} {Γ γ : ZFSet} {A A' B B' : ZFSet -> ZFSet} 
+  (HA : ∀ γ ∈ Γ, A γ ∈ 𝕌 nA) (HB : ∀ γa ∈ ctxExt nA Γ A, B γa ∈ 𝕌 nB)
+  (HA' : ∀ γ ∈ Γ, A' γ ∈ 𝕌 nA') (HB' : ∀ γa ∈ ctxExt nA' Γ A', B' γa ∈ 𝕌 nB')
+  (Hγ : γ ∈ Γ) (H : piTy_HO nA nB A B γ ≡ piTy_HO nA' nB' A' B' γ) :
+  typeToGraph nA nB (A γ) (fun a => B ⟨ γ ; a ⟩) ≡ typeToGraph nA nB' (A γ) (fun a => B' ⟨ γ ; a ⟩).
+Proof.
+  set (N := maxmax nA nA' nB nB').
+  pose proof (piTy_HO_inj_dom HA HB HA' HB' Hγ H) as HAA'.
+  pose proof (piTy_HO_inj_dom_level HA HB HA' HB' Hγ H) as HnAA'. destruct HnAA'.
+  refine (trans (b := cod_piTy_set N (piTy_HO nA nB A B γ)) _ _).
+  { symmetry. refine (cod_piTy_set_eq _ _ HA HB Hγ) ; apply (maxmax_le nA nA nB nB'). }
+  refine (trans (fequal (cod_piTy_set N) H) _).
+  refine (transpS (fun X => _ ≡ typeToGraph nA nB' X _) (sym HAA') _).
+  refine (cod_piTy_set_eq _ _ HA' HB' Hγ) ; apply (maxmax_le nA nA nB nB').
+Qed.
+
+Lemma piTy_HO_inj_cod {nA nA' nB nB' : nat} {Γ γ a : ZFSet} {A A' B B' : ZFSet -> ZFSet} 
+  (HA : ∀ γ ∈ Γ, A γ ∈ 𝕌 nA) (HB : ∀ γa ∈ ctxExt nA Γ A, B γa ∈ 𝕌 nB)
+  (HA' : ∀ γ ∈ Γ, A' γ ∈ 𝕌 nA') (HB' : ∀ γa ∈ ctxExt nA' Γ A', B' γa ∈ 𝕌 nB')
+  (Hγ : γ ∈ Γ) (H : piTy_HO nA nB A B γ ≡ piTy_HO nA' nB' A' B' γ) (Ha : a ∈ 𝕌el nA (A γ)) :
   B ⟨ γ ; a ⟩ ≡ B' ⟨ γ ; a ⟩.
 Proof.
-  pose proof (piTy_HO_inj1 HA HB HA' HB' Hγ H) as HAA'.
-  pose proof (piTy_HO_inj2' HA HB HA' HB' Hγ H) as HBB'.
-  refine (trans (b := setAppArr (𝕌el n (A γ)) (𝕌 n) (typeToGraph n (A γ) (fun a => B ⟨ γ ; a ⟩)) a) _ _).
+  pose proof (piTy_HO_inj_dom HA HB HA' HB' Hγ H) as HAA'.
+  pose proof (piTy_HO_inj_dom_level HA HB HA' HB' Hγ H) as HnAA'. destruct HnAA'.
+  pose proof (piTy_HO_inj_cod' HA HB HA' HB' Hγ H) as HBB'.
+  pose proof (piTy_HO_inj_cod_level HA HB HA' HB' Hγ H) as HnBB'. destruct HnBB'.
+  refine (trans (b := setAppArr (𝕌el nA (A γ)) (𝕌 nB) (typeToGraph nA nB (A γ) (fun a => B ⟨ γ ; a ⟩)) a) _ _).
   { symmetry. refine (trans _ _). apply setAppArr_HO ; try assumption.
     now apply (typeExt_typing HA HB). reflexivity. }
-  refine (trans (fequal (fun X => setAppArr (𝕌el n (A γ)) (𝕌 n) X a) HBB') _).
+  refine (trans (fequal (fun X => setAppArr (𝕌el nA (A γ)) (𝕌 nB) X a) HBB') _).
   refine (trans _ _). apply setAppArr_HO ; try assumption. 2:reflexivity.
-  intros a' Ha'. pose proof (transpS (fun X => a' ∈ 𝕌el n X) HAA' Ha') as Ha''. cbn in Ha''. clear Ha'.
+  intros a' Ha'. pose proof (transpS (fun X => a' ∈ 𝕌el nA X) HAA' Ha') as Ha''. cbn in Ha''. clear Ha'.
   revert a' Ha''. now apply (typeExt_typing HA' HB').
 Qed.
 
 (* Lambda abstraction *)
 
-Definition lamTm_HO (n : nat) (A t : ZFSet -> ZFSet) : ZFSet -> ZFSet :=
-  fun γ => relToGraph (𝕌el n (A γ)) (𝕍 n) (HO_rel (fun a => t ⟨ γ ; a ⟩)).
+Definition lamTm_HO (nA nB : nat) (A t : ZFSet -> ZFSet) : ZFSet -> ZFSet :=
+  fun γ => relToGraph (𝕌el nA (A γ)) (𝕍 (max nA nB)) (HO_rel (fun a => t ⟨ γ ; a ⟩)).
 
-Lemma lamTm_HO_typing (n : nat) {Γ : ZFSet} {A B t : ZFSet -> ZFSet}
-  (HA : ∀ γ ∈ Γ, A γ ∈ 𝕌 n) (HB : ∀ γa ∈ ctxExt n Γ A, B γa ∈ 𝕌 n)
-  (Ht : ∀ γa ∈ ctxExt n Γ A, t γa ∈ 𝕌el n (B γa)) :
-  ∀ γ ∈ Γ, lamTm_HO n A t γ ∈ 𝕌el n (piTy_HO n A B γ).
+Lemma lamTm_HO_typing {nA nB : nat} {Γ : ZFSet} {A B t : ZFSet -> ZFSet}
+  (HA : ∀ γ ∈ Γ, A γ ∈ 𝕌 nA) (HB : ∀ γa ∈ ctxExt nA Γ A, B γa ∈ 𝕌 nB)
+  (Ht : ∀ γa ∈ ctxExt nA Γ A, t γa ∈ 𝕌el nB (B γa)) :
+  ∀ γ ∈ Γ, lamTm_HO nA nB A t γ ∈ 𝕌el (max nA nB) (piTy_HO nA nB A B γ).
 Proof.
   intros γ Hγ. cbn. refine (transpS (fun X => _ ∈ X) (sym (el_piTy HA HB Hγ)) _). apply ZFincomp. split.
   - apply relToGraph_typing. apply HO_rel_typing.
     intros a Ha. eapply ZFuniv_trans. now apply (termExt_typing HA HB Ht).
-    apply 𝕌el_typing. now apply (typeExt_typing HA HB).
-  - intros a Ha. refine (transpS (fun X => X ∈ 𝕌el n (B ⟨ γ ; a ⟩)) _ (Ht ⟨ γ ; a ⟩ _)).
+    eapply univ_le_incl. apply Nat.le_max_r. apply 𝕌el_typing. now apply (typeExt_typing HA HB).
+  - intros a Ha. refine (transpS (fun X => X ∈ 𝕌el nB (B ⟨ γ ; a ⟩)) _ (Ht ⟨ γ ; a ⟩ _)).
     + refine (sym _). refine (trans _ _). apply setAppArr_HO ; [ | assumption].
-      intros a' Ha'. eapply ZFuniv_trans. now apply (termExt_typing HA HB Ht). apply 𝕌el_typing.
-      now apply (typeExt_typing HA HB). reflexivity.
+      intros a' Ha'. eapply ZFuniv_trans. now apply (termExt_typing HA HB Ht).
+      eapply univ_le_incl. apply Nat.le_max_r. apply 𝕌el_typing. now apply (typeExt_typing HA HB).
+      reflexivity.
     + apply setMkSigma_typing ; try assumption. intros γ' Hγ'. apply 𝕌el_typing. now apply HA.
 Qed.
 
 (* Application *)
 
-Definition appTm_HO (n : nat) (A t u : ZFSet -> ZFSet) : ZFSet -> ZFSet :=
-  fun γ => setAppArr (𝕌el n (A γ)) (𝕍 n) (t γ) (u γ).
+Definition appTm_HO (nA nB : nat) (A t u : ZFSet -> ZFSet) : ZFSet -> ZFSet :=
+  fun γ => setAppArr (𝕌el nA (A γ)) (𝕍 (max nA nB)) (t γ) (u γ).
 
-Lemma appTm_HO_typing (n : nat) {Γ : ZFSet} {A B t u : ZFSet -> ZFSet} 
-  (HA : ∀ γ ∈ Γ, A γ ∈ 𝕌 n) (HB : ∀ γa ∈ ctxExt n Γ A, B γa ∈ 𝕌 n)
-  (Ht : ∀ γ ∈ Γ, t γ ∈ 𝕌el n (piTy_HO n A B γ)) (Hu : ∀ γ ∈ Γ, u γ ∈ 𝕌el n (A γ)) :
-  ∀ γ ∈ Γ, appTm_HO n A t u γ ∈ 𝕌el n (B ⟨ γ ; u γ ⟩).
+Lemma appTm_HO_typing {nA nB : nat} {Γ : ZFSet} {A B t u : ZFSet -> ZFSet} 
+  (HA : ∀ γ ∈ Γ, A γ ∈ 𝕌 nA) (HB : ∀ γa ∈ ctxExt nA Γ A, B γa ∈ 𝕌 nB)
+  (Ht : ∀ γ ∈ Γ, t γ ∈ 𝕌el (max nA nB) (piTy_HO nA nB A B γ)) (Hu : ∀ γ ∈ Γ, u γ ∈ 𝕌el nA (A γ)) :
+  ∀ γ ∈ Γ, appTm_HO nA nB A t u γ ∈ 𝕌el nB (B ⟨ γ ; u γ ⟩).
 Proof.
-  intros γ Hγ. assert (t γ ∈ setPi n (𝕌el n (A γ)) (fun a => 𝕌el n (B ⟨ γ ; a ⟩))) as Htγ.
+  intros γ Hγ. assert (t γ ∈ setPi (max nA nB) (𝕌el nA (A γ)) (fun a => 𝕌el nB (B ⟨ γ ; a ⟩))) as Htγ.
   { refine (transpS (fun X => t γ ∈ X) _ (Ht γ Hγ)). now apply (el_piTy (Γ := Γ)). }
   cbn. unfold appTm_HO. apply ZFincomp in Htγ. destruct Htγ as [ _ H ].
   apply H. now apply Hu.
@@ -151,44 +263,37 @@ Qed.
 
 (* Equations (β and η) *)
 
-Lemma piTy_HO_β (n : nat) {Γ : ZFSet} {A B t u : ZFSet -> ZFSet} 
-  (HA : ∀ γ ∈ Γ, A γ ∈ 𝕌 n) (HB : ∀ γa ∈ ctxExt n Γ A, B γa ∈ 𝕌 n)
-  (Ht : ∀ γa ∈ ctxExt n Γ A, t γa ∈ 𝕌el n (B γa)) (Hu : ∀ γ ∈ Γ, u γ ∈ 𝕌el n (A γ)) :
-  ∀ γ ∈ Γ, appTm_HO n A (lamTm_HO n A t) u γ ≡ t ⟨ γ ; u γ ⟩.
+Lemma piTy_HO_β {nA nB : nat} {Γ : ZFSet} {A B t u : ZFSet -> ZFSet} 
+  (HA : ∀ γ ∈ Γ, A γ ∈ 𝕌 nA) (HB : ∀ γa ∈ ctxExt nA Γ A, B γa ∈ 𝕌 nB)
+  (Ht : ∀ γa ∈ ctxExt nA Γ A, t γa ∈ 𝕌el nB (B γa)) (Hu : ∀ γ ∈ Γ, u γ ∈ 𝕌el nA (A γ)) :
+  ∀ γ ∈ Γ, appTm_HO nA nB A (lamTm_HO nA nB A t) u γ ≡ t ⟨ γ ; u γ ⟩.
 Proof.
   intros γ Hγ. cbn. refine (trans _ _). apply setAppArr_HO ; try assumption. 3:reflexivity.
-  - intros a Ha. eapply ZFuniv_trans. now apply (termExt_typing HA HB Ht). apply 𝕌el_typing.
-    now apply (typeExt_typing HA HB).
+  - intros a Ha. eapply ZFuniv_trans. now apply (termExt_typing HA HB Ht).
+    eapply univ_le_incl. apply Nat.le_max_r. apply 𝕌el_typing. now apply (typeExt_typing HA HB).
   - now apply Hu.
 Qed.
 
-(* Γ ⊢ t : Π A B *)
-
-(* Γ , A ⊢ wk t : Π (wk A) (wk1 B) *)
-(* Γ , A ⊢ 0 : wk A *)
-(* Γ , A ⊢ (wk t) @ 0 : wk1 B [ 0 ] = B *)
-(* Γ ⊢ λ (wk t) @ 0 : Π A B *)
-
-Lemma piTy_HO_η (n : nat) {Γ : ZFSet} {A B t u : ZFSet -> ZFSet}
-  (HA : ∀ γ ∈ Γ, A γ ∈ 𝕌 n) (HB : ∀ γa ∈ ctxExt n Γ A, B γa ∈ 𝕌 n)
-  (Ht : ∀ γ ∈ Γ, t γ ∈ 𝕌el n (piTy_HO n A B γ)) :
-  ∀ γ ∈ Γ, t γ ≡ lamTm_HO n A (appTm_HO n (fun γa => A (ctx_wk n Γ A γa)) (fun γa => t (ctx_wk n Γ A γa)) (ctx_var0 n Γ A)) γ.
+Lemma piTy_HO_η {nA nB : nat} {Γ : ZFSet} {A B t u : ZFSet -> ZFSet}
+  (HA : ∀ γ ∈ Γ, A γ ∈ 𝕌 nA) (HB : ∀ γa ∈ ctxExt nA Γ A, B γa ∈ 𝕌 nB)
+  (Ht : ∀ γ ∈ Γ, t γ ∈ 𝕌el (max nA nB) (piTy_HO nA nB A B γ)) :
+  ∀ γ ∈ Γ, t γ ≡ lamTm_HO nA nB A (appTm_HO nA nB (fun γa => A (ctx_wk nA Γ A γa)) (fun γa => t (ctx_wk nA Γ A γa)) (ctx_var0 nA Γ A)) γ.
 Proof.
   intros γ Hγ. cbn. unfold lamTm_HO. unfold appTm_HO.
-  assert (t γ ∈ setPi n (𝕌el n (A γ)) (fun a => 𝕌el n (B ⟨ γ ; a ⟩))) as Ht'.
+  assert (t γ ∈ setPi (max nA nB) (𝕌el nA (A γ)) (fun a => 𝕌el nB (B ⟨ γ ; a ⟩))) as Ht'.
   { refine (transpS (fun X => t γ ∈ X) (el_piTy HA HB Hγ) _). now apply Ht. }
   apply ZFincomp in Ht'. destruct Ht' as [ Ht' _ ].
-  apply (setArr_funext (A := 𝕌el n (A γ)) (B := 𝕍 n)).
+  apply (setArr_funext (A := 𝕌el nA (A γ)) (B := 𝕍 (max nA nB))).
   - exact Ht'.
   - apply relToGraph_typing. apply HO_rel_typing. intros a Ha.
-    refine (transp2S (fun X Y => setAppArr (𝕌el n (A X)) (𝕍 n) (t X) Y ∈ 𝕍 n)
+    refine (transp2S (fun X Y => setAppArr (𝕌el nA (A X)) (𝕍 (max nA nB)) (t X) Y ∈ 𝕍 (max nA nB))
               (sym (ctxExtβ1 HA Hγ Ha)) (sym (ctxExtβ2 HA Hγ Ha)) _).
     apply setAppArr_typing. 2:assumption. exact Ht'.
   - intros a Ha. refine (sym _). refine (trans _ _). apply setAppArr_HO. 2:assumption.
     + clear a Ha. intros a Ha. 
-      refine (transp2S (fun X Y => setAppArr (𝕌el n (A X)) (𝕍 n) (t X) Y ∈ 𝕍 n)
+      refine (transp2S (fun X Y => setAppArr (𝕌el nA (A X)) (𝕍 (max nA nB)) (t X) Y ∈ 𝕍 (max nA nB))
                 (sym (ctxExtβ1 HA Hγ Ha)) (sym (ctxExtβ2 HA Hγ Ha)) _).
       apply setAppArr_typing. 2:assumption. exact Ht'.
-    + refine (fequal2 (fun X Y => setAppArr (𝕌el n (A X)) (𝕍 n) (t X) Y)
+    + refine (fequal2 (fun X Y => setAppArr (𝕌el nA (A X)) (𝕍 (max nA nB)) (t X) Y)
                 ((ctxExtβ1 HA Hγ Ha)) ((ctxExtβ2 HA Hγ Ha))).
 Qed.
