theories/SetModel/HO_nat.v
@@ -67,36 +67,36 @@ Definition natrecTm_HO (n : nat) (P pz ps m : ZFSet -> ZFSet) : ZFSet -> ZFSet :
   fun γ => natrec2 n (fun m => 𝕌el n (P ⟨ γ ; m ⟩)) (pz γ) (fun m pm => ps ⟨ ⟨ γ ; m ⟩ ; pm ⟩) (m γ).
 
 Lemma natrecTm_HO_typing_aux {n : nat} {Γ γ : ZFSet} {P ps : ZFSet -> ZFSet}
-  (HP : ∀ γm ∈ ctxExt n Γ natTy_HO, P γm ∈ 𝕌 n)
-  (Hps : ∀ γmp ∈ ctxExt n (ctxExt n Γ natTy_HO) P,
-      ps γmp ∈ 𝕌el n (P ⟨ ctx_wk n Γ natTy_HO (ctx_wk n (ctxExt n Γ natTy_HO) P γmp)
-                        ; sucTm_HO (fun γmp => ctx_var0 n Γ natTy_HO (ctx_wk n (ctxExt n Γ natTy_HO) P γmp)) γmp ⟩))
+  (HP : ∀ γm ∈ ctxExt 0 Γ natTy_HO, P γm ∈ 𝕌 n)
+  (Hps : ∀ γmp ∈ ctxExt n (ctxExt 0 Γ natTy_HO) P,
+      ps γmp ∈ 𝕌el n (P ⟨ ctx_wk 0 Γ natTy_HO (ctx_wk n (ctxExt 0 Γ natTy_HO) P γmp)
+                        ; sucTm_HO (fun γmp => ctx_var0 0 Γ natTy_HO (ctx_wk n (ctxExt 0 Γ natTy_HO) P γmp)) γmp ⟩))
   (Hγ : γ ∈ Γ) :
   ∀ x ∈ ω, ∀ px ∈ 𝕌el n (P ⟨ γ ; x ⟩), ps ⟨ ⟨ γ ; x ⟩ ; px ⟩ ∈ 𝕌el n (P ⟨ γ ; ZFsuc x ⟩).
 Proof.
   intros x Hx px Hpx.
-  assert (x ∈ 𝕌el n (natTy_HO γ)).
+  assert (x ∈ 𝕌el 0 (natTy_HO γ)).
   { exact (transpS (fun X => x ∈ X) (sym el_natTy) Hx). }
-  assert (⟨ ⟨ γ; x ⟩; px ⟩ ∈ ctxExt n (ctxExt n Γ natTy_HO) P) as H0.
+  assert (⟨ ⟨ γ; x ⟩; px ⟩ ∈ ctxExt n (ctxExt 0 Γ natTy_HO) P) as H0.
   { apply setMkSigma_typing ; try assumption. intros y Hy. apply 𝕌el_typing. now apply HP.
     apply setMkSigma_typing ; try assumption. intros y Hy. apply 𝕌el_typing. now apply (natTy_HO_typing (Γ := Γ)). }
   specialize (Hps _ H0). cbn in Hps. refine (transp2S (fun X Y => _ ∈ 𝕌el n (P ⟨ X ; Y ⟩)) _ _ Hps).
-  + refine (trans (fequal (ctx_wk n Γ natTy_HO) _) _).
+  + refine (trans (fequal (ctx_wk 0 Γ natTy_HO) _) _).
     * apply ctxExtβ1 ; try assumption. apply setMkSigma_typing ; try assumption.
       intros y Hy. apply 𝕌el_typing. now apply (natTy_HO_typing (Γ := Γ)).
     * apply ctxExtβ1 ; try assumption. now apply natTy_HO_typing.
-  + unfold sucTm_HO. refine (fequal ZFsuc _). refine (trans (fequal (ctx_var0 n Γ natTy_HO) _) _).
+  + unfold sucTm_HO. refine (fequal ZFsuc _). refine (trans (fequal (ctx_var0 0 Γ natTy_HO) _) _).
     * apply ctxExtβ1 ; try assumption. apply setMkSigma_typing ; try assumption.
       intros y Hy. apply 𝕌el_typing. now apply (natTy_HO_typing (Γ := Γ)).
     * apply ctxExtβ2 ; try assumption. now apply natTy_HO_typing.
 Qed.
 
 Lemma natrecTm_HO_typing {n : nat} {Γ : ZFSet} {P pz ps m : ZFSet -> ZFSet}
-  (HP : ∀ γm ∈ ctxExt n Γ natTy_HO, P γm ∈ 𝕌 n) (Hpz : ∀ γ ∈ Γ, pz γ ∈ 𝕌el n (P ⟨ γ ; zeroTm_HO γ ⟩))
-  (Hps : ∀ γmp ∈ ctxExt n (ctxExt n Γ natTy_HO) P,
-      ps γmp ∈ 𝕌el n (P ⟨ ctx_wk n Γ natTy_HO (ctx_wk n (ctxExt n Γ natTy_HO) P γmp)
-                        ; sucTm_HO (fun γmp => ctx_var0 n Γ natTy_HO (ctx_wk n (ctxExt n Γ natTy_HO) P γmp)) γmp ⟩))
-  (Hm : ∀ γ ∈ Γ, m γ ∈ 𝕌el n (natTy_HO γ)) :
+  (HP : ∀ γm ∈ ctxExt 0 Γ natTy_HO, P γm ∈ 𝕌 n) (Hpz : ∀ γ ∈ Γ, pz γ ∈ 𝕌el n (P ⟨ γ ; zeroTm_HO γ ⟩))
+  (Hps : ∀ γmp ∈ ctxExt n (ctxExt 0 Γ natTy_HO) P,
+      ps γmp ∈ 𝕌el n (P ⟨ ctx_wk 0 Γ natTy_HO (ctx_wk n (ctxExt 0 Γ natTy_HO) P γmp)
+                        ; sucTm_HO (fun γmp => ctx_var0 0 Γ natTy_HO (ctx_wk n (ctxExt 0 Γ natTy_HO) P γmp)) γmp ⟩))
+  (Hm : ∀ γ ∈ Γ, m γ ∈ 𝕌el 0 (natTy_HO γ)) :
   ∀ γ ∈ Γ, natrecTm_HO n P pz ps m γ ∈ 𝕌el n (P ⟨ γ ; m γ ⟩).
 Proof.
   intros γ Hγ. cbn. unfold natrecTm_HO. apply (natrec2_typing (P := fun m => 𝕌el n (P ⟨ γ ; m ⟩))).
@@ -108,10 +108,10 @@ Proof.
 Qed.
 
 Lemma natrecTm_HO_β1 {n : nat} {Γ : ZFSet} {P pz ps : ZFSet -> ZFSet}
-  (HP : ∀ γm ∈ ctxExt n Γ natTy_HO, P γm ∈ 𝕌 n) (Hpz : ∀ γ ∈ Γ, pz γ ∈ 𝕌el n (P ⟨ γ ; zeroTm_HO γ ⟩))
-  (Hps : ∀ γmp ∈ ctxExt n (ctxExt n Γ natTy_HO) P,
-      ps γmp ∈ 𝕌el n (P ⟨ ctx_wk n Γ natTy_HO (ctx_wk n (ctxExt n Γ natTy_HO) P γmp)
-                        ; sucTm_HO (fun γmp => ctx_var0 n Γ natTy_HO (ctx_wk n (ctxExt n Γ natTy_HO) P γmp)) γmp ⟩)) :
+  (HP : ∀ γm ∈ ctxExt 0 Γ natTy_HO, P γm ∈ 𝕌 n) (Hpz : ∀ γ ∈ Γ, pz γ ∈ 𝕌el n (P ⟨ γ ; zeroTm_HO γ ⟩))
+  (Hps : ∀ γmp ∈ ctxExt n (ctxExt 0 Γ natTy_HO) P,
+      ps γmp ∈ 𝕌el n (P ⟨ ctx_wk 0 Γ natTy_HO (ctx_wk n (ctxExt 0 Γ natTy_HO) P γmp)
+                        ; sucTm_HO (fun γmp => ctx_var0 0 Γ natTy_HO (ctx_wk n (ctxExt 0 Γ natTy_HO) P γmp)) γmp ⟩)) :
   ∀ γ ∈ Γ, natrecTm_HO n P pz ps zeroTm_HO γ ≡ pz γ.
 Proof.
   intros γ Hγ. cbn. unfold natrecTm_HO. unfold zeroTm_HO. apply natrec2_β1.
@@ -122,11 +122,11 @@ Proof.
 Qed.
 
 Lemma natrecTm_HO_β2 {n : nat} {Γ : ZFSet} {P pz ps m : ZFSet -> ZFSet}
-  (HP : ∀ γm ∈ ctxExt n Γ natTy_HO, P γm ∈ 𝕌 n) (Hpz : ∀ γ ∈ Γ, pz γ ∈ 𝕌el n (P ⟨ γ ; zeroTm_HO γ ⟩))
-  (Hps : ∀ γmp ∈ ctxExt n (ctxExt n Γ natTy_HO) P,
-      ps γmp ∈ 𝕌el n (P ⟨ ctx_wk n Γ natTy_HO (ctx_wk n (ctxExt n Γ natTy_HO) P γmp)
-                        ; sucTm_HO (fun γmp => ctx_var0 n Γ natTy_HO (ctx_wk n (ctxExt n Γ natTy_HO) P γmp)) γmp ⟩))
-  (Hm : ∀ γ ∈ Γ, m γ ∈ 𝕌el n (natTy_HO γ)) :
+  (HP : ∀ γm ∈ ctxExt 0 Γ natTy_HO, P γm ∈ 𝕌 n) (Hpz : ∀ γ ∈ Γ, pz γ ∈ 𝕌el n (P ⟨ γ ; zeroTm_HO γ ⟩))
+  (Hps : ∀ γmp ∈ ctxExt n (ctxExt 0 Γ natTy_HO) P,
+      ps γmp ∈ 𝕌el n (P ⟨ ctx_wk 0 Γ natTy_HO (ctx_wk n (ctxExt 0 Γ natTy_HO) P γmp)
+                        ; sucTm_HO (fun γmp => ctx_var0 0 Γ natTy_HO (ctx_wk n (ctxExt 0 Γ natTy_HO) P γmp)) γmp ⟩))
+  (Hm : ∀ γ ∈ Γ, m γ ∈ 𝕌el 0 (natTy_HO γ)) :
   ∀ γ ∈ Γ, natrecTm_HO n P pz ps (sucTm_HO m) γ ≡ ps ⟨ ⟨ γ ; m γ ⟩ ; natrecTm_HO n P pz ps m γ ⟩.
 Proof.
   intros γ Hγ. cbn. unfold natrecTm_HO. unfold sucTm_HO. refine (trans _ _).
