theories/SetModel/HO_obseq.v
@@ -1,3 +1,4 @@
+From Stdlib Require Import Arith.
 Require Import library.
 Require Import ZF_axioms ZF_library ZF_nat.
 Require Import HO HO_prop HO_univ HO_forall HO_nat HO_pi.
@@ -65,25 +66,25 @@ Qed.
 
 Definition funextTm_HO (A B f g e : ZFSet -> ZFSet) : ZFSet -> ZFSet := fun _ => ∅.
 
-Lemma funextTm_HO_typing {n : nat} {Γ : ZFSet} {A B f g e : ZFSet -> ZFSet}
-  (HA : ∀ γ ∈ Γ, A γ ∈ 𝕌 n) (HB : ∀ γa ∈ ctxExt n Γ A, B γa ∈ 𝕌 n)
-  (Hf : ∀ γ ∈ Γ, f γ ∈ 𝕌el n (piTy_HO n A B γ)) (Hg : ∀ γ ∈ Γ, g γ ∈ 𝕌el n (piTy_HO n A B γ))
-  (He : ∀ γa ∈ ctxExt n Γ A,
-      e γa ∈ eqTy_HO B (appTm_HO n (fun γa => A (ctx_wk n Γ A γa)) (fun γa => f (ctx_wk n Γ A γa)) (ctx_var0 n Γ A))
-                       (appTm_HO n (fun γa => A (ctx_wk n Γ A γa)) (fun γa => g (ctx_wk n Γ A γa)) (ctx_var0 n Γ A)) γa) :
-  ∀ γ ∈ Γ, funextTm_HO A B f g e γ ∈ eqTy_HO (piTy_HO n A B) f g γ.
+Lemma funextTm_HO_typing {nA nB : nat} {Γ : ZFSet} {A B f g e : ZFSet -> ZFSet}
+  (HA : ∀ γ ∈ Γ, A γ ∈ 𝕌 nA) (HB : ∀ γa ∈ ctxExt nA Γ A, B γa ∈ 𝕌 nB)
+  (Hf : ∀ γ ∈ Γ, f γ ∈ 𝕌el (max nA nB) (piTy_HO nA nB A B γ)) (Hg : ∀ γ ∈ Γ, g γ ∈ 𝕌el (max nA nB) (piTy_HO nA nB A B γ))
+  (He : ∀ γa ∈ ctxExt nA Γ A,
+      e γa ∈ eqTy_HO B (appTm_HO nA nB (fun γa => A (ctx_wk nA Γ A γa)) (fun γa => f (ctx_wk nA Γ A γa)) (ctx_var0 nA Γ A))
+                       (appTm_HO nA nB (fun γa => A (ctx_wk nA Γ A γa)) (fun γa => g (ctx_wk nA Γ A γa)) (ctx_var0 nA Γ A)) γa) :
+  ∀ γ ∈ Γ, funextTm_HO A B f g e γ ∈ eqTy_HO (piTy_HO nA nB A B) f g γ.
 Proof.
   intros γ Hγ. unfold funextTm_HO. unfold eqTy_HO. apply prop_true_iff.
-  apply (setArr_funext (A := 𝕌el n (A γ)) (B := 𝕍 n)).
+  apply (setArr_funext (A := 𝕌el nA (A γ)) (B := 𝕍 (max nA nB))).
   - pose proof (transpS (fun X => f γ ∈ X) (el_piTy HA HB Hγ) (Hf γ Hγ)) as H. apply ZFincomp in H. now destruct H.
   - pose proof (transpS (fun X => g γ ∈ X) (el_piTy HA HB Hγ) (Hg γ Hγ)) as H. apply ZFincomp in H. now destruct H.
-  - intros a Ha. assert (⟨ γ ; a ⟩ ∈ ctxExt n Γ A) as Hγa.
+  - intros a Ha. assert (⟨ γ ; a ⟩ ∈ ctxExt nA Γ A) as Hγa.
     { apply setMkSigma_typing ; try assumption. intros γ' Hγ'. apply 𝕌el_typing. now apply HA. }
     specialize (He _ Hγa). apply prop_true_if in He. refine (trans (sym _) (trans He _)).
-    + refine (fequal2 (fun X Y => setAppArr (𝕌el n (A X)) (𝕍 n) (f X) Y) _ _).
+    + refine (fequal2 (fun X Y => setAppArr (𝕌el nA (A X)) (𝕍 (max nA nB)) (f X) Y) _ _).
       * now apply ctxExtβ1.
       * now apply ctxExtβ2.
-    + refine (fequal2 (fun X Y => setAppArr (𝕌el n (A X)) (𝕍 n) (g X) Y) _ _).
+    + refine (fequal2 (fun X Y => setAppArr (𝕌el nA (A X)) (𝕍 (max nA nB)) (g X) Y) _ _).
       * now apply ctxExtβ1.
       * now apply ctxExtβ2.
 Qed.
@@ -105,88 +106,88 @@ Qed.
 
 Definition piinj1Tm_HO (A A' B B' e : ZFSet -> ZFSet) : ZFSet -> ZFSet := fun _ => ∅.
 
-Lemma piinj1Tm_HO_typing {n : nat} {Γ : ZFSet} {A A' B B' e : ZFSet -> ZFSet}
-  (HA : ∀ γ ∈ Γ, A γ ∈ 𝕌 n) (HB : ∀ γa ∈ ctxExt n Γ A, B γa ∈ 𝕌 n)
-  (HA' : ∀ γ ∈ Γ, A' γ ∈ 𝕌 n) (HB' : ∀ γa ∈ ctxExt n Γ A', B' γa ∈ 𝕌 n)
-  (He : ∀ γ ∈ Γ, e γ ∈ eqTy_HO (univTy_HO n) (piTy_HO n A B) (piTy_HO n A' B') γ)
-  : ∀ γ ∈ Γ, piinj1Tm_HO A A' B B' e γ ∈ eqTy_HO (univTy_HO n) A' A γ.
+Lemma piinj1Tm_HO_typing {nA nB : nat} {Γ : ZFSet} {A A' B B' e : ZFSet -> ZFSet}
+  (HA : ∀ γ ∈ Γ, A γ ∈ 𝕌 nA) (HB : ∀ γa ∈ ctxExt nA Γ A, B γa ∈ 𝕌 nB)
+  (HA' : ∀ γ ∈ Γ, A' γ ∈ 𝕌 nA) (HB' : ∀ γa ∈ ctxExt nA Γ A', B' γa ∈ 𝕌 nB)
+  (He : ∀ γ ∈ Γ, e γ ∈ eqTy_HO (univTy_HO (max nA nB)) (piTy_HO nA nB A B) (piTy_HO nA nB A' B') γ)
+  : ∀ γ ∈ Γ, piinj1Tm_HO A A' B B' e γ ∈ eqTy_HO (univTy_HO (max nA nB)) A' A γ.
 Proof.
   intros γ Hγ. cbn. unfold eqTy_HO. unfold piinj1Tm_HO. apply prop_true_iff. apply sym.
-  apply (piTy_HO_inj1 HA HB HA' HB' Hγ). specialize (He γ Hγ). unfold eqTy_HO in He.
+  apply (piTy_HO_inj_dom HA HB HA' HB' Hγ). specialize (He γ Hγ). unfold eqTy_HO in He.
   now apply prop_true_if in He.
 Qed.
 
 Definition piinj2Tm_HO (A A' B B' e a : ZFSet -> ZFSet) : ZFSet -> ZFSet := fun _ => ∅.
 
-Lemma piinj2Tm_HO_typing {n : nat} {Γ : ZFSet} {A A' B B' e a : ZFSet -> ZFSet}
-  (HA : ∀ γ ∈ Γ, A γ ∈ 𝕌 n) (HB : ∀ γa ∈ ctxExt n Γ A, B γa ∈ 𝕌 n)
-  (HA' : ∀ γ ∈ Γ, A' γ ∈ 𝕌 n) (HB' : ∀ γa ∈ ctxExt n Γ A', B' γa ∈ 𝕌 n)
-  (He : ∀ γ ∈ Γ, e γ ∈ eqTy_HO (univTy_HO n) (piTy_HO n A B) (piTy_HO n A' B') γ)
-  (Ha : ∀ γ ∈ Γ, a γ ∈ 𝕌el n (A' γ)) (a0 := castTm_HO A' A (piinj1Tm_HO A A' B B' e) a)
-  : ∀ γ ∈ Γ, piinj2Tm_HO A A' B B' e a γ ∈ eqTy_HO (univTy_HO n) (fun γ => B ⟨ γ ; a0 γ ⟩) (fun γ => B' ⟨ γ ; a γ ⟩) γ.
+Lemma piinj2Tm_HO_typing {nA nB : nat} {Γ : ZFSet} {A A' B B' e a : ZFSet -> ZFSet}
+  (HA : ∀ γ ∈ Γ, A γ ∈ 𝕌 nA) (HB : ∀ γa ∈ ctxExt nA Γ A, B γa ∈ 𝕌 nB)
+  (HA' : ∀ γ ∈ Γ, A' γ ∈ 𝕌 nA) (HB' : ∀ γa ∈ ctxExt nA Γ A', B' γa ∈ 𝕌 nB)
+  (He : ∀ γ ∈ Γ, e γ ∈ eqTy_HO (univTy_HO (max nA nB)) (piTy_HO nA nB A B) (piTy_HO nA nB A' B') γ)
+  (Ha : ∀ γ ∈ Γ, a γ ∈ 𝕌el nA (A' γ)) (a0 := castTm_HO A' A (piinj1Tm_HO A A' B B' e) a)
+  : ∀ γ ∈ Γ, piinj2Tm_HO A A' B B' e a γ ∈ eqTy_HO (univTy_HO (max nA nB)) (fun γ => B ⟨ γ ; a0 γ ⟩) (fun γ => B' ⟨ γ ; a γ ⟩) γ.
 Proof.
   intros γ Hγ. cbn. unfold piinj2Tm_HO. unfold eqTy_HO. apply prop_true_iff.
   unfold castTm_HO in a0. unfold a0. clear a0. specialize (He γ Hγ). unfold eqTy_HO in He.
-  apply prop_true_if in He. assert (a γ ∈ 𝕌el n (A γ)).
-  { refine (transpS (fun X => a γ ∈ 𝕌el n X) _ (Ha γ Hγ)). apply sym.
-    now apply (piTy_HO_inj1 HA HB HA' HB' Hγ). }
-  apply (piTy_HO_inj2 HA HB HA' HB' Hγ He H).
+  apply prop_true_if in He. assert (a γ ∈ 𝕌el nA (A γ)).
+  { refine (transpS (fun X => a γ ∈ 𝕌el nA X) _ (Ha γ Hγ)). apply sym.
+    now apply (piTy_HO_inj_dom HA HB HA' HB' Hγ). }
+  apply (piTy_HO_inj_cod HA HB HA' HB' Hγ He H).
 Qed.
 
 (* Computation rule for cast on pi
    Since cast is the identity, this rule is just η, modulo a bit of transport *)
 
-Lemma castTm_HO_pi {n : nat} {Γ : ZFSet} {A A' B B' e f : ZFSet -> ZFSet}
-  (HA : ∀ γ ∈ Γ, A γ ∈ 𝕌 n) (HB : ∀ γa ∈ ctxExt n Γ A, B γa ∈ 𝕌 n)
-  (HA' : ∀ γ ∈ Γ, A' γ ∈ 𝕌 n) (HB' : ∀ γa ∈ ctxExt n Γ A', B' γa ∈ 𝕌 n)
-  (He : ∀ γ ∈ Γ, e γ ∈ eqTy_HO (univTy_HO n) (piTy_HO n A B) (piTy_HO n A' B') γ)
-  (Hf : ∀ γ ∈ Γ, f γ ∈ 𝕌el n (piTy_HO n A B γ))
-  (Au := fun γa => A (ctx_wk n Γ A' γa)) (A'u := fun γa => A' (ctx_wk n Γ A' γa))
-  (Bu := fun γaa => B ⟨ ctx_wk n Γ A' (ctx_wk n (ctxExt n Γ A') Au γaa) ; ctx_var0 n (ctxExt n Γ A') Au γaa ⟩)
-  (B'u := fun γaa => B' ⟨ ctx_wk n Γ A' (ctx_wk n (ctxExt n Γ A') A'u γaa) ; ctx_var0 n (ctxExt n Γ A') A'u γaa ⟩)
-  (t1 := castTm_HO A'u Au (piinj1Tm_HO Au A'u Bu B'u (fun γa => e (ctx_wk n Γ A' γa))) (fun γa => ctx_var0 n Γ A' γa))
-  (t2 := appTm_HO n Au (fun γa => f (ctx_wk n Γ A' γa)) t1)
-  (t3 := castTm_HO (fun γa => B ⟨ ctx_wk n Γ A' γa ; t1 γa ⟩) B'
-           (piinj2Tm_HO Au A'u Bu B'u (fun γa => e (ctx_wk n Γ A' γa)) (fun γa => ctx_var0 n Γ A' γa)) t2)
-  (t4 := lamTm_HO n A' t3) : ∀ γ ∈ Γ, castTm_HO (piTy_HO n A B) (piTy_HO n A' B') e f γ ≡ t4 γ.
+Lemma castTm_HO_pi {nA nB : nat} {Γ : ZFSet} {A A' B B' e f : ZFSet -> ZFSet}
+  (HA : ∀ γ ∈ Γ, A γ ∈ 𝕌 nA) (HB : ∀ γa ∈ ctxExt nA Γ A, B γa ∈ 𝕌 nB)
+  (HA' : ∀ γ ∈ Γ, A' γ ∈ 𝕌 nA) (HB' : ∀ γa ∈ ctxExt nA Γ A', B' γa ∈ 𝕌 nB)
+  (He : ∀ γ ∈ Γ, e γ ∈ eqTy_HO (univTy_HO (max nA nB)) (piTy_HO nA nB A B) (piTy_HO nA nB A' B') γ)
+  (Hf : ∀ γ ∈ Γ, f γ ∈ 𝕌el (max nA nB) (piTy_HO nA nB A B γ))
+  (Au := fun γa => A (ctx_wk nA Γ A' γa)) (A'u := fun γa => A' (ctx_wk nA Γ A' γa))
+  (Bu := fun γaa => B ⟨ ctx_wk nA Γ A' (ctx_wk nA (ctxExt nA Γ A') Au γaa) ; ctx_var0 nA (ctxExt nA Γ A') Au γaa ⟩)
+  (B'u := fun γaa => B' ⟨ ctx_wk nA Γ A' (ctx_wk nA (ctxExt nA Γ A') A'u γaa) ; ctx_var0 nA (ctxExt nA Γ A') A'u γaa ⟩)
+  (t1 := castTm_HO A'u Au (piinj1Tm_HO Au A'u Bu B'u (fun γa => e (ctx_wk nA Γ A' γa))) (fun γa => ctx_var0 nA Γ A' γa))
+  (t2 := appTm_HO nA nB Au (fun γa => f (ctx_wk nA Γ A' γa)) t1)
+  (t3 := castTm_HO (fun γa => B ⟨ ctx_wk nA Γ A' γa ; t1 γa ⟩) B'
+           (piinj2Tm_HO Au A'u Bu B'u (fun γa => e (ctx_wk nA Γ A' γa)) (fun γa => ctx_var0 nA Γ A' γa)) t2)
+  (t4 := lamTm_HO nA nB A' t3) : ∀ γ ∈ Γ, castTm_HO (piTy_HO nA nB A B) (piTy_HO nA nB A' B') e f γ ≡ t4 γ.
 Proof.
   intros γ Hγ. unfold castTm_HO in *. unfold t4. unfold t3. unfold t2. unfold t1. unfold Au.
   clear t1 t2 t3 t4. unfold lamTm_HO. unfold appTm_HO.
   specialize (He γ Hγ). unfold eqTy_HO in He. apply prop_true_if in He.
-  assert (A γ ≡ A' γ) as HAA'. { now apply (piTy_HO_inj1 HA HB HA' HB' Hγ). }
-  assert (f γ ∈ setPi n (𝕌el n (A' γ)) (fun a => 𝕌el n (B' ⟨ γ ; a ⟩))) as Hf'.
+  assert (A γ ≡ A' γ) as HAA'. { now apply (piTy_HO_inj_dom HA HB HA' HB' Hγ). }
+  assert (f γ ∈ setPi (max nA nB) (𝕌el nA (A' γ)) (fun a => 𝕌el nB (B' ⟨ γ ; a ⟩))) as Hf'.
   { refine (transpS (fun X => f γ ∈ X) (el_piTy HA' HB' Hγ) _).
-    refine (transpS (fun X => f γ ∈ 𝕌el n X) He _). now apply Hf. }
+    refine (transpS (fun X => f γ ∈ 𝕌el (max nA nB) X) He _). now apply Hf. }
   apply ZFincomp in Hf'. destruct Hf' as [ Hf' _ ].
-  apply (setArr_funext (A := 𝕌el n (A' γ)) (B := 𝕍 n)).
+  apply (setArr_funext (A := 𝕌el nA (A' γ)) (B := 𝕍 (max nA nB))).
   - exact Hf'.
   - apply relToGraph_typing. apply HO_rel_typing. intros a Ha.
-    refine (transp2S (fun X Y => setAppArr (𝕌el n (A X)) (𝕍 n) (f X) Y ∈ 𝕍 n)
+    refine (transp2S (fun X Y => setAppArr (𝕌el nA (A X)) (𝕍 (max nA nB)) (f X) Y ∈ 𝕍 (max nA nB))
               (sym (ctxExtβ1 HA' Hγ Ha)) (sym (ctxExtβ2 HA' Hγ Ha)) _).
-    refine (transpS (fun X => setAppArr (𝕌el n X) (𝕍 n) (f γ) a ∈ 𝕍 n) (sym HAA') _).
+    refine (transpS (fun X => setAppArr (𝕌el nA X) (𝕍 (max nA nB)) (f γ) a ∈ 𝕍 (max nA nB)) (sym HAA') _).
     apply setAppArr_typing. 2:assumption. exact Hf'.
   - intros a Ha. refine (sym _). refine (trans _ _). apply setAppArr_HO. 2:assumption.
     + clear a Ha. intros a Ha. 
-      refine (transp2S (fun X Y => setAppArr (𝕌el n (A X)) (𝕍 n) (f X) Y ∈ 𝕍 n)
+      refine (transp2S (fun X Y => setAppArr (𝕌el nA (A X)) (𝕍 (max nA nB)) (f X) Y ∈ 𝕍 (max nA nB))
                 (sym (ctxExtβ1 HA' Hγ Ha)) (sym (ctxExtβ2 HA' Hγ Ha)) _).
-      refine (transpS (fun X => setAppArr (𝕌el n X) (𝕍 n) (f γ) a ∈ 𝕍 n) (sym HAA') _).
+      refine (transpS (fun X => setAppArr (𝕌el nA X) (𝕍 (max nA nB)) (f γ) a ∈ 𝕍 (max nA nB)) (sym HAA') _).
       apply setAppArr_typing. 2:assumption. exact Hf'.
-    + refine (fequal2 (fun X Y => setAppArr (𝕌el n (A X)) (𝕍 n) (f X) Y)
+    + refine (fequal2 (fun X Y => setAppArr (𝕌el nA (A X)) (𝕍 (max nA nB)) (f X) Y)
                 ((ctxExtβ1 HA' Hγ Ha)) ((ctxExtβ2 HA' Hγ Ha))).
 Qed.
 
 (* No-confusion theorems. Copy and paste for all type formers if necessary *)
 
-Lemma nat_neq_pi {n : nat} {Γ : ZFSet} {A B e : ZFSet -> ZFSet}
-  (HA : ∀ γ ∈ ⋆, A γ ∈ 𝕌 n) (HB : ∀ γa ∈ ctxExt n ⋆ A, B γa ∈ 𝕌 n)
-  (He : ∀ γ ∈ ⋆, e γ ∈ eqTy_HO (univTy_HO n) natTy_HO (piTy_HO n A B) γ) : FalseS.
+Lemma nat_neq_pi {nA nB : nat} {Γ : ZFSet} {A B e : ZFSet -> ZFSet}
+  (HA : ∀ γ ∈ ⋆, A γ ∈ 𝕌 nA) (HB : ∀ γa ∈ ctxExt nA ⋆ A, B γa ∈ 𝕌 nB)
+  (He : ∀ γ ∈ ⋆, e γ ∈ eqTy_HO (univTy_HO (max nA nB)) natTy_HO (piTy_HO nA nB A B) γ) : FalseS.
 Proof.
   assert (∅ ∈ ⋆) as H. { now apply inSetSingl. }
   specialize (He _ H). cbn in He. unfold eqTy_HO in He. apply prop_true_if in He.
   assert (ZFzero ≡ ZFone).
-  { refine (trans (sym _) (trans (fequal (𝕌hd n) He) _)).
+  { refine (trans (sym _) (trans (fequal (𝕌hd (max nA nB)) He) _)).
     - now apply hd_natTy.
-    - now apply (hd_piTy HA HB H). }
+    - refine (hd_piTy' _ _ HA HB H). apply Nat.le_max_l. apply Nat.le_max_r. }
   now apply (zero_ne_suc ∅).
 Qed.
 
